Added clean_expression simproc to Encoding.thy (was in Test.thy).
In Test.thy: Code for showing <= for expressions.

src/main/isabelle/Test.thy
@@ -1,66 +1,67 @@
 theory Test
-  imports Real_Sqrt2 Encoding Tactics QRHL_Code 
+  imports Encoding Tactics QRHL_Code "~~/src/HOL/Eisbach/Eisbach_Tools"
 begin
 
-lemma  "CNOT \<cdot> ((hadamard \<cdot> ket 0) \<otimes> ket 0) = EPR"
+
+
+
+(* 
+lemma "hadamard\<guillemotright>\<lbrakk>q1\<rbrakk> \<cdot> Qeq[q1=q2] = hadamard\<guillemotright>\<lbrakk>q2\<rbrakk> \<cdot> Qeq[q1=q2]"
   apply (auto simp: prepare_for_code)
   apply eval
+  done
 
-(* definition "matrix_H = mat_of_rows_list 2 [ [sqrt 2::complex, sqrt 2], [sqrt 2, -sqrt 2] ]"
-axiomatization where bounded_of_mat_H[code]: "mat_of_bounded hadamard = matrix_H"
-
-value "hadamard" *)
-
-
-
-
-
-
-
-variables quantum q :: bit and quantum r :: bit begin
-term "hadamard\<guillemotright>\<lbrakk>q\<rbrakk>"
-lemma "space_div (span{ket 0}\<guillemotright>\<lbrakk>q\<rbrakk>) (ket 1) \<lbrakk>r\<rbrakk> = span{ket 0}\<guillemotright>\<lbrakk>q\<rbrakk>"
+ *)  
+  
+  
+  
+(* lemma "space_div (span{ket 0}\<guillemotright>\<lbrakk>q\<rbrakk>) (ket 1) \<lbrakk>r\<rbrakk> = span{ket 0}\<guillemotright>\<lbrakk>q\<rbrakk>"
   apply (auto simp: prepare_for_code)
   by eval
 
 lemma "space_div (span{ket (0,0), ket(1,1)}\<guillemotright>\<lbrakk>q,r\<rbrakk>) (ket 0) \<lbrakk>r\<rbrakk> = span{ket 0}\<guillemotright>\<lbrakk>q\<rbrakk>"
   apply (auto simp: prepare_for_code)
   by eval
+ *)
 
-end
 
-ML {*
-fun is_explicit_expression (Const(@{const_name expression},_) $ Q $ _) =
-  ((QRHL.parse_varterm Q; true) handle TERM _ => false)
-  | is_explicit_expression _ = false
-fun is_varlist_explicit_expression (Const(@{const_name expression},_) $ Q $ _) =
-  ((QRHL.parse_varlist Q; true) handle TERM _ => false)
-  |  is_varlist_explicit_expression _ = false
-*}
-
-ML {*
-fun clean_expression_simproc _ ctxt ct = 
-  let val t = Thm.term_of ct in
-  if is_explicit_expression t andalso not (is_varlist_explicit_expression t) then
-      SOME (Encoding.clean_expression_conv ctxt ct) handle CTERM _ => NONE
-    else
-      NONE
-  end
-*}
-
-simproc_setup clean_expression ("expression Q e") = clean_expression_simproc
+axiomatization eval_variable :: "'a variable \<Rightarrow> mem2 \<Rightarrow> 'a"
+axiomatization eval_variables :: "'a variables \<Rightarrow> mem2 \<Rightarrow> 'a"
+axiomatization where
+  eval_variables_unit: "eval_variables \<lbrakk>\<rbrakk> m = ()"
+and eval_variables_singleton: "eval_variables \<lbrakk>q\<rbrakk> m = eval_variable q m"
+and eval_variables_concat: "eval_variables (variable_concat Q R) m = (eval_variables Q m, eval_variables R m)"
+for q :: "'a variable" and Q :: "'b variables" and R :: "'c variables" 
 
 
 instantiation expression :: (ord) ord begin
-instance sorry
+definition "less_eq_expression e f \<longleftrightarrow> expression_eval e \<le> expression_eval f"
+definition "less_expression e f \<longleftrightarrow> expression_eval e \<le> expression_eval f \<and> \<not> (expression_eval f \<le> expression_eval e)"
+instance by intro_classes
 end
 
+axiomatization where expression_eval: "expression_eval (expression Q e) m = e (eval_variables Q m)"
 
-ML {*
+instantiation expression :: (preorder) preorder begin
+instance apply intro_classes
+  unfolding less_expression_def less_eq_expression_def 
+  using order_trans by auto
+end
+
+(* ML {*
   fun subst_expression_simproc _ ctxt ct = SOME (Encoding.subst_expression_conv ctxt ct) handle CTERM _ => NONE
-*}
+*} *)
 
-simproc_setup subst_expression ("subst_expression (substitute1 x (expression R f')) (expression Q e')") = subst_expression_simproc
+(* simproc_setup subst_expression ("subst_expression (substitute1 x (expression R f')) (expression Q e')") = subst_expression_simproc *)
+
+
+
+lemma qrhl_top: "qrhl A p1 p2 (expression Q (\<lambda>z. top))" sorry
+lemma qrhl_top': "f \<ge> top \<Longrightarrow> qrhl A p1 p2 (expression Q f)" sorry
+
+
+lemma tmp: "(\<And>x. C x) \<Longrightarrow> (C x)" 
+  by metis
 
 
 variables
@@ -70,12 +71,6 @@ variables
   classical c :: int and
   quantum q :: int
 begin
-
-lemma qrhl_top: "qrhl A p1 p2 (expression Q (\<lambda>z. top))" sorry
-lemma qrhl_top': "f \<ge> top \<Longrightarrow> qrhl A p1 p2 (expression Q f)" sorry
-
-
-
 
 lemma
   assumes [simp]: "x\<ge>0"
@@ -91,26 +86,72 @@ lemma skip:
   shows "qrhl A [] [] B"
   sorry
 
+(* lemma expression_leq:
+  assumes "\<And>x. e x \<le> e' x"
+  shows "expression X e \<le> expression X e'"
+  using assms unfolding less_eq_expression_def expression_eval le_fun_def
+  by auto *)
+
+(* 
 lemma expression_leq1:
   assumes "\<And>x. e x \<le> e' x"
   shows "expression \<lbrakk>v\<rbrakk> e \<le> expression \<lbrakk>v\<rbrakk> e'"
-  sorry
+  using assms by (rule expression_leq) 
 
 lemma expression_leq2:
   assumes "\<And>x y. e x y \<le> e' x y"
   shows "expression \<lbrakk>v,w\<rbrakk> (\<lambda>(x,y). e x y) \<le> expression \<lbrakk>v,w\<rbrakk> (\<lambda>(x,y). e' x y)"
-  sorry
+  apply (rule expression_leq) using assms by auto
+ *)
 
+ML \<open>
+fun rename_tac_variant names = SUBGOAL (fn (goal,i) =>
+  let val used = Term.add_free_names goal []
+      val fresh = Name.variant_list used names
+  in
+    rename_tac fresh i
+  end)
+\<close>
+
+method_setup rename_tac_eisbach = \<open>
+  Args.term >> (fn name => fn ctxt => 
+    case name of Free(name',_) => SIMPLE_METHOD' (rename_tac_variant [name'])
+               | _ => (warning ("Could not convert "^Syntax.string_of_term ctxt name^" into a variable name. Not renaming."); Method.succeed)
+    )\<close>
+
+
+method intro_expression_leq = 
+  (rule less_eq_expression_def[THEN iffD2],
+   rule le_fun_def[THEN iffD2],
+   match conclusion in "\<forall>mem::mem2. C mem" for C \<Rightarrow>
+      \<open>rule allI, rename_tac mem, 
+       match conclusion in "C mem" for mem \<Rightarrow> 
+         \<open>unfold expression_eval[where m=mem],
+          unfold eval_variables_concat[where m=mem] eval_variables_unit[where m=mem] eval_variables_singleton[where m=mem],
+          unfold case_prod_conv,
+          (match conclusion in "PROP (D (eval_variable v mem))" for D v \<Rightarrow> 
+              \<open>rule meta_spec[where x="eval_variable v mem" and P=D], rename_tac_eisbach v\<close>)+
+         \<close>
+      \<close>
+  )[1]
+
+
+lemma test:
+  (* assumes "\<And>x y. e x \<le> e' x y" *)
+  shows "Expr[a-b*b] \<le> Expr[a]"
+  (* apply (insert assms)   *)
+  apply intro_expression_leq 
+  by auto
 
 schematic_goal
   assumes [simp]: "x\<ge>0"
   shows "qrhl Expr[ Cla[x1=0 \<and> x2=1] ] [qinit \<lbrakk>q\<rbrakk> Expr[ ket 0 ] ] [assign var_x Expr[x-1] ] Expr[ Cla[x1\<ge>x2] ]"
-  using [[method_error,show_types]]
+  using [[method_error]]
   apply (tactic \<open>Tactics.wp_tac @{context} true 1\<close>) 
   apply (tactic \<open>Tactics.wp_tac @{context} false 1\<close>)
   apply simp
   apply (rule skip)
-  apply (rule expression_leq2)
+  apply intro_expression_leq
   by simp
 
 end
